src/ecParsetree.ml
@@ -1273,6 +1273,8 @@ type threquire =
 type pbind_bitstring =
   { from_ : pqsymbol
   ; to_   : pqsymbol
+  ; toint : pqsymbol
+  ; ofint : pqsymbol
   ; type_ : pty
   ; size  : EcBigInt.zint }
   
